Definitions/Values.v
@@ -1,32 +1,26 @@
+From stdpp Require Import gmap.
+Require Import Ascii String.
 Require Import Definitions.Regions.
-Require Import Definitions.Keys.
 Require Import Definitions.Expressions.
 Require Import Definitions.ComputedActions.
-
-Module E := FMapAVL.Make (AsciiVars).
-Module Raw := E.Raw.
-
 
 Inductive Val :=
 | Loc  : Region_in_Expr -> nat -> Val
 | Num  : nat -> Val
 | Bit  : bool -> Val
-| Cls  : (Raw.t Val * Rho * Expr) -> Val
+| Cls  : (gmap VarId Val * Rho * Expr) -> Val
 | Eff  : Theta -> Val
 | Unit : Val
 | Pair : Val * Val -> Val.
 
+Definition Env := gmap VarId Val.
 
-Definition Env := Raw.t Val.
-Definition V_Key := Raw.key.
+Definition find_E (k: VarId) (m: Env) : option Val := m !! k.
 
-
-Definition find_E (k: VarId) (m: Env) : option Val := Raw.find (elt := Val) k m. 
-
-Definition update_E (p: VarId * Val) (m : Env) := Raw.add (fst p) (snd p) m.
+Definition update_E (p: VarId * Val) (m: Env) :=  <[ fst p := snd p ]>  m.
 
 Definition update_rec_E (f : VarId * Val) (x: VarId * Val) m :=
-  let m' := Raw.add (fst f) (snd f) m
-  in Raw.add (fst x) (snd x) m'.
+  let m' := update_E f m
+  in update_E x m'.
 
 
